

\documentclass[10pt]{article}

\usepackage{graphicx}
\usepackage{fancybox}
\usepackage{epsfig}
\usepackage{float}
\usepackage{amsmath,amsfonts,amssymb}
\usepackage{subfigure}
\usepackage{multirow}
\usepackage{bm}
\usepackage[]{algorithm2e}
\usepackage{color}

\input{mydef}

\parskip 2.0mm
\topmargin  -2.0cm
\textwidth 16cm
\textheight 22.5cm
\topmargin -1.5cm
\oddsidemargin 0mm

\title{CS6316 Homework 02: The Bias-variance Tradeoff, SVMs and Kernel Methods}
\author{Gabriel Hanson}
\date{Due on Oct. 27, 2022 11:59 PM}

% ***************************************************
\begin{document} 
\maketitle

\begin{enumerate}
\item \textbf{Bias-Variance Tradeoff} (12 points)

Please refer to the attached iPython notebook file.

\pagebreak
\item \textbf{KKT Conditions} (4 points) The Lagrangian form of SVMs with slack variable $\vec{\xi}$ is formulated as
  \begin{equation}
    \label{eq:non-sep-svm}
    \begin{split}
      L(\vw,b,\bm{\xi},\bm{\alpha},\bm{\beta})= & \frac{1}{2}\|\vw\|_2^2 + C\sum_{i=1}^{m}\xi_i\\
      & -\sum_{i=1}^{m}\alpha_i(y_i(\trans{\vw}\vx_i+b)-1+\xi_i)\\
      & - \sum_{i=1}^{m}\beta_i\xi_i
    \end{split}
  \end{equation}
  Similar to SVMs in separable cases (page 19), to find the KKT conditions (as in page 29, we need to compute the derivative with respect to all parameters $\{\vw,b,\bm{\xi},\bm{\alpha},\bm{\beta}\}$. Overall, please show that the KKT conditions can be represented to the following equations
  \begin{eqnarray}
    \vw &=& \sum_{i=1}^{m}{\alpha_i}y_i\vx_i\\
    \sum_{i=1}^{m}\alpha_iy_i &=& 0 \\
    \alpha_i + \beta_i &=& C\\
    \alpha_i = 0 &\text{or}& y_i(\trans{\vw}\vx_i + b) = 1 - \xi_i\\
    \beta_i = 0 &\text{or}& \xi_i = 0
  \end{eqnarray}
\hspace{\parindent}\textit{\textbf{Solution:}}

$$  \frac{\partial L}{\partial \vw} = \vw - \sum_{i=1}^{m} \alpha_i y_i x_i  = 0 \quad \quad \longrightarrow  \quad \vw = \sum_{i=1}^{m} \alpha_i y_i x_i $$

$$ \frac{\partial L}{\partial b} = - \sum_{i=1}^{m} \alpha_i y_i = 0 \quad \quad \longrightarrow \quad \alpha_i y_i = 0  $$

$$ \frac{\partial L}{\partial {\xi}}  = C - \sum_{i=1}^{m} \alpha_i - \sum_{i=1}^{m} \beta_i = 0 \quad \quad \longrightarrow \quad C = \alpha_i + \beta_i $$

and 

$$ \forall i \quad \alpha_i(y_i(\vw^\intercal \vx_i + b) -1 + \xi_i = 0 \quad \quad \longrightarrow \quad \quad \alpha_i = 0 \quad \text{or} \quad y_i(\vw^\intercal \vx_i + b) = 1 - \xi_i  $$

$$ \forall i \quad \beta_i\xi_i = 0 \quad \quad \longrightarrow \quad \quad \beta_i = 0 \quad \text{or} \quad \xi_i = 0 $$


\pagebreak
\item \textbf{Kernel Methods} (4 points) In our lecture, we show that a special case of the polynomial kernels
  \begin{equation}
    K(\vx,\vx') = (\dotp{\vx}{\vx'} + c)^d
  \end{equation}
  with $d=2$ and $\vx,\vx'\in\mathbb{R}^2$.
  On page 53 of the slides, we should how this special case can be decomposed as a dot product with a nonlinear mapping $\Phi(\cdot)$
  \begin{equation}
    K(\vx,\vx') = \dotp{\Phi(\vx)}{\Phi(\vx')}.
  \end{equation}
  In this problem, consider $d=3$ with $\vx,\vx'\in\mathbb{R}^2$ and show how the $\Phi(\vx)$ is defined in this case. 
\end{enumerate}

\hspace{\parindent}\textit{\textbf{Solution:}}

$$ K(\vx,\vx') = (\dotp{\vx}{\vx'} + c)^3 \;\forall \  x,x^\prime \in\mathbb{R}^2 $$
$$ K(\vx,\vx') = (\dotp{\vx}{\vx'} + c)^2 * (\dotp{\vx}{\vx'} + c) $$
$$ = ({x_1}{x_1'}  + {x_2}{x_2'}  + c)^2 * ({x_1}{x_1'}  + {x_2}{x_2'}  + c)$$
This first term was solved for in slide 56 of the SVM lecture, which I will substitute in here
$$  = ({x_1^2}{x_1'^2} + {x_2^2}{x_2'^2}  +  2{x_1}{x_1'}{x_2}{x_2'}  + 2c{x_1}{x_1'} + 2c{x_2}{x_2'}+c^2 )* ({x_1}{x_1'}  + {x_2}{x_2'}  + c)$$
$$ = ({x_1^3}{x_1'^3} + {x_1}{x_1'}{x_2^2}{x_2'^2} + 2{x_1^2}{x_1'^2}{x_2}{x_2'} +  2c{x_1^2}{x_1'^2} + 2c{x_1}{x_1'}{x_2}{x_2'} + c^2 {x_1}{x_1'} $$
$$ + \; {x_1^2}{x_1'^2}{x_2}{x_2'} + {x_2^3}{x_2'^3} + 2{x_1}{x_1'}{x_2^2}{x_2'^2} + 2c{x_1}{x_1'}{x_2}{x_2'}  + 2c{x_2^2}{x_2'^2} + c^2 {x_2}{x_2'} $$
$$ +  \;c{x_1^2}{x_1'^2} + c{x_2^2}{x_2'^2} + 2c{x_1}{x_1'}{x_2}{x_2'} + 2c^2{x_1}{x_1'} + 2c^2{x_2}{x_2'} + c^3 )$$
Combining terms here leaves us with
$$ = ({x_1^3}{x_1'^3} + {x_2^3}{x_2'^3}  + 3{x_1^2}{x_1'^2}{x_2}{x_2'} + 3{x_1}{x_1'}{x_2^2}{x_2'^2} + 3 c{x_1^2}{x_1'^2} +  3c{x_2^2}{x_2'^2} + 6c{x_1}{x_1'}{x_2}{x_2'} + 3c^2{x_1}{x_1'} + 3c^2{x_2}{x_2'} + c^3 ) $$
which can be rewritten as

\def\A{
\begin{bmatrix}
    {x_1^3} , {x_2^3} , {\sqrt{3}{x_1^2}x_2} , {\sqrt{3}{x_1}x_2^2} , {\sqrt{3c}x_1^2} , {\sqrt{3c}x_2^2} ,{\sqrt{6c}{x_1}x_2} , {\sqrt{3}cx_1} ,  {\sqrt{3}cx_2} , c^{3/2}
\end{bmatrix}}

\def\B{
\begin{bmatrix}
	x_1'^3 \\
     	x_2'^3 \\
    	\sqrt{3}{x_1'^2}x_2' \\
	\sqrt{3}{x_1'}x_2'^2 \\
        	\sqrt{3c}x_1'^2 \\
	\sqrt{3c}x_2'^2 \\
	\sqrt{6c}{x_1'}x_2' \\
	\sqrt{3}cx_1' \\
	\sqrt{3}cx_2' \\
	c^{3/2}
\end{bmatrix}}


\begin{align*}
\A \B
\end{align*}



Let \( K(\vx,\vx') = \dotp{\phi(\vx)}{\phi(\vx')} \), then

$$ \phi(\vx)  = [ {x_1^3} , {x_2^3} , {\sqrt{3}{x_1^2}x_2} , {\sqrt{3}{x_1}x_2^2} , {\sqrt{3c}x_1^2} , {\sqrt{3c}x_2^2} ,{\sqrt{6c}{x_1}x_2} , {\sqrt{3}cx_1} ,  {\sqrt{3}cx_2} , c^{3/2}]^\intercal $$ 

% *******************END OF DOCUMENT*****************
\end{document}

